output/first.ec
@@ -1,91 +1,47 @@
-require import AllCore.
+require import List AllCore.
 require import List.
-
-prover quorum=2 ["Z3" "Alt-Ergo"].
-
 module M2 = {
-  var l : bool list
+  var l_2b8920 : bool list
   var s1, s2 : bool list
   var r : bool
   var i : int
 
   proc compare() : bool = {
- l <- [];
+  l_2b8920 <- []; 
   r <- false;
   i <- 0;
 
   while(i < size s1){
-  l <- true::l;
+  l_2b8920 <- true::l_2b8920;
         r <- (nth (false) s1 i = nth (false) s2 i) || r;
         i <- i + 1;
     }
- l <- false::l
+ l_2b8920 <- false::l_2b8920;
         return r;
   }
 }.
-
-lemma fixed_compare (_s1 _s2 : bool list):
-equiv[M2.compare ~ M2.compare : size M2.s1{1} = size M2.s2{1} /\
-      size M2.s1{2} = size M2.s2{2} /\ size M2.s1{1} = size M2.s1{2}
-      ==> ={M2.l}].
-    proof.
-    proc.    
- l <- [];
-    while(={M2.l, M2.i} /\ size M2.s1{1} = size M2.s2{1} /\
-  l <- true::l;
- l <- false::l
-      size M2.s1{2} = size M2.s2{2} /\ size M2.s1{1} = size M2.s1{2});auto;smt().
-  qed.
-
-           
 module M1 = {
-  var l : bool list
+  var l_2b8920 : bool list
   var s1, s2 : bool list
   var r : bool
   var i : int
   
   proc compare() : bool = {
- l <- [];
+  l_2b8920 <- []; 
   r <- true;
   i <- 0;
     
   while (i < size s1){
-  l <- true::l;
+  l_2b8920 <- true::l_2b8920;
       if (nth (true) s1 i = nth (true) s2 i){
- l <- true::l;
+ l_2b8920 <- true::l_2b8920;
       }else{
- l <- false::l;
+l_2b8920 <- false::l_2b8920;
           r <- false;
       }
       i <- i + 1;
     }
- l <- false::l
+ l_2b8920 <- false::l_2b8920;
     return r;
   }
 }.
-
-(* The precondition is that the length of the bitstrings are always of equal 
-length. The postcondition is that l{1} and l{2} are always equal length. It seems
-like to be totally secure they should be equal but since the program is branching
-on private data, l depends on private data. *)
-lemma compare (_s1 _s2 : bool list):
-equiv[M1.compare ~ M1.compare : size M1.s1{1} = size M1.s2{1} /\
-    size M1.s1{2} = size M1.s2{2} /\ size M1.s1{1} = size M1.s1{2}
-      ==> size M1.l{1} = size M1.l{2}]. 
-    proof.
-      proc.
- l <- [];
-      auto;auto.
-    while(={M1.i} /\ size M1.s1{1} = size M1.s1{2} /\ 
-  l <- true::l;
- l <- false::l
-      size M1.s1{1} = size M1.s2{1} /\ size M1.s1{2} = size M1.s2{2} /\
-      M1.i{1} <= size M1.s1{1} /\ size M1.l{1} = size M1.l{2}).
-      auto.
-    smt().
-      auto.
-      smt(size_ge0).
-qed.
-
-
-
