input/insertionsort.ec
@@ -1,0 +1,25 @@
+    require import AllCore List.
+    prover quorum=2 ["Z3" "Alt-Ergo"].
+
+
+    module M1 = {
+    
+
+    proc isort(a : int list) : int list = {
+        var i,j,x : int;
+        i <- 1;
+
+        while (i < size a){
+            j <- i;
+            while(0 < j &&  nth (-1) a (j) < (nth (-1) a (j-1))){
+                x <- nth (-1) a j;
+                a <- take (j-2) a ++ [x] ++ [nth (-1) a (j - 1)] ++ drop (j) a;
+                j <- j - 1; 
+            }
+            i <- i + 1;
+        }
+
+        return a;
+    }
+    
+    }.
