proofs/first.ec
@@ -1,0 +1,61 @@
+require import AllCore.
+require import List.
+
+prover quorum=2 ["Z3" "Alt-Ergo"].
+
+module M2 = {
+  var s1, s2 : bool list
+  var l : bool list
+  var r : bool
+  var i : int
+
+  proc compare() : bool = {
+  r <- false;
+  i <- 0;
+  l <- [];
+
+  while(i < size s1){
+        l <- true::l;
+        r <- (nth (false) s1 i = nth (false) s2 i) || r;
+        i <- i + 1;
+    }
+        return r;
+  }
+}.
+
+lemma fixed_compare (_s1 _s2 : bool list):
+equiv[M2.compare ~ M2.compare : size M2.s1{1} = size M2.s2{1} /\
+      size M2.s1{2} = size M2.s2{2} /\ size M2.s1{1} = size M2.s1{2}
+      ==> ={M2.l}].
+    proof.
+    proc.    
+    while(={M2.l, M2.i} /\ size M2.s1{1} = size M2.s2{1} /\
+      size M2.s1{2} = size M2.s2{2} /\ size M2.s1{1} = size M2.s1{2});auto;smt().
+  qed.
+
+           
+module M1 = {
+  var s1, s2 : bool list
+  var l : bool list
+  var r : bool
+  var i : int
+  
+  proc compare() : bool = {
+  r <- true;
+  i <- 0;
+  l <- [];
+    
+  while (i < size s1){
+  l <- true::l;
+      if (nth (true) s1 i = nth (true) s2 i){
+          l <- true::l;
+      }else{
+          l <- false::l;
+          r <- false;
+      }
+      i <- i + 1;
+    }
+        l <- false::l;
+    return r;
+  }
+}.
