proofs/relationalsecure.ec
@@ -1,0 +1,48 @@
+require import AllCore List.
+prover quorum=2 ["Z3" "Alt-Ergo"].
+
+
+module M1 = {
+  var l_df77cf : bool list
+
+  proc min(a : int list) : int = {
+  var y, i : int;
+  l_df77cf <- [];
+  i <- 1;
+  y <- nth 0 a 0;
+
+  while(i < size a){
+    l_df77cf <- true::l_df77cf;
+    if(nth 0 a i < y){
+      l_df77cf <- true::l_df77cf;
+      y <- nth 0 a i;
+    }
+    else{
+          l_df77cf <- false::l_df77cf;
+    }
+      i <- i + 1;
+    }
+      l_df77cf <- false::l_df77cf;
+      return y;
+  }
+}.
+
+lemma secureMin:
+equiv [M1.min ~ M1.min : size a{1} = size a{2} /\ 1 <= size a{1} /\ 
+    forall(x, c: int), 0 <= x <= size a{1} /\ 0 <= c <= size a{1} =>
+      (nth 0 a{1} x < nth 0 a{1} c <=> nth 0 a{2} x < nth 0 a{2} c) 
+      ==> ={M1.l_df77cf}].
+        proc.
+        seq 3 3 : (={i, M1.l_df77cf} /\ size a{1} = size a{2} /\ 1 <= size a{1} /\
+           (forall(x, c: int), 0 <= x <= size a{1} /\ 0 <= c <= size a{1} =>
+      (nth 0 a{1} x < nth 0 a{1} c <=> nth 0 a{2} x < nth 0 a{2} c)) /\
+    i{1} = 1 /\ M1.l_df77cf{1} = [] /\
+    y{1} = nth 0 a{1} 0 /\ y{2} = nth 0 a{2} 0);auto.
+
+    while(={i, M1.l_df77cf} /\ 0 < i{1} /\  size a{1} = size a {2} /\
+        (forall(x, c: int), 0 <= x <= size a{1} /\ 0 <= c <= size a{1} =>
+      (nth 0 a{1} x < nth 0 a{1} c <=> nth 0 a{2} x < nth 0 a{2} c)) /\
+        i{1} <= size a{1} /\ ((forall(k: int), (0 <= k <= size a{1} =>
+          (nth 0 a{1} k < y{1} <=> nth 0 a{2} k < y{2})))));auto;smt().
+        
+  qed.
