proofs/timing2.ec
@@ -1,0 +1,103 @@
+require import AllCore IntDiv List.
+
+prover quorum=2 ["Z3" "Alt-Ergo"].
+
+module M1 = {
+  var c_f9da02 : int
+  var r : bool
+  var i : int
+
+  proc test() : int = {
+  c_f9da02 <- 0;
+
+  i <- 10;
+
+  if(r){
+  i <- i - 10;
+  c_f9da02 <- c_f9da02 + 1;
+    }else{
+        i <- i + 10;
+        c_f9da02 <- c_f9da02 + 1;
+    }
+
+        return i;
+  }
+}.
+
+lemma test:
+equiv[M1.test ~ M1.test :
+     true ==> ={M1.c_f9da02}].
+    proof.
+      proc.
+      auto.
+  qed.
+
+
+
+  module M2 = {
+    var c_fa9d65 : int
+    var r : bool
+    var i : int
+
+    proc test() : int = {
+    var j : int;
+    var cnt : int;
+    c_fa9d65 <- 0;
+
+    cnt <- 0;
+    j <- 0;
+
+    while(j < i){
+    cnt <- cnt + 10;
+    c_fa9d65 <- c_fa9d65 + 1;
+    j <- j + 1;
+    c_fa9d65 <- c_fa9d65 + 1;
+      }
+
+          j <- 0;
+          while(j < (100 - i)){
+          cnt <- cnt - 10;
+          c_fa9d65 <- c_fa9d65 + 1;
+          j <- j + 1;
+          c_fa9d65 <- c_fa9d65 + 1;
+      }
+
+
+          return i;
+    }
+    }.
+
+lemma test2:
+equiv[M2.test ~ M2.test :
+     0 < M2.i{1} < 100 /\ 0 < M2.i{2} < 100 ==> ={M2.c_fa9d65}].
+    proof.
+      proc.
+      seq 3 3 : (={cnt, j, M2.c_fa9d65} /\  0 < M2.i{1} < 100 /\ 0 < M2.i{2} < 100
+      /\ cnt{1} = 0 /\ j{1} = 0 /\ M2.c_fa9d65{1}  = 0).
+      auto.
+      while {1} ( 0 < M2.i{1} < 100 /\ 0 < M2.i{2} < 100 /\
+      M2.c_fa9d65{1} = M2.i{1} * 2 + j{1} * 2 /\ 
+      0 <= j{1} <= (100 - M2.i{1})) ((100 - M2.i{1} - j{1})).
+      auto;smt().
+
+      while {2} ( 0 < M2.i{1} < 100 /\ 0 < M2.i{2} < 100 /\
+      M2.c_fa9d65{2} = M2.i{2} * 2 + j{2} * 2 /\ 
+      0 <= j{2} <= (100 - M2.i{2})) ((100 - M2.i{2} - j{2})).
+      auto;smt().
+
+     auto.
+
+      while {1} ( 0 < M2.i{1} < 100 /\ 0 < M2.i{2} < 100 /\
+      M2.c_fa9d65{1} = j{1} * 2 /\ 
+      0 <= j{1} <= (M2.i{1})) ((M2.i{1} - j{1})).
+      auto;smt().
+
+      while {2} ( 0 < M2.i{1} < 100 /\ 0 < M2.i{2} < 100 /\
+      M2.c_fa9d65{2} = j{2} * 2 /\ 
+      0 <= j{2} <= (M2.i{2})) ((M2.i{2} - j{2})).
+      auto;smt().
+
+      skip;smt().
+
+  qed.
+  
